coq-osiris/examples/splay.v
@@ -386,179 +386,181 @@ Lemma Splay__spec:
 Proof.
   intros.
   pure1.
-  pure_specify "splay" splay_spec.
-  (* Subgoal: prove that [splay] satisfies its specification. *)
-  { generalize η; clear η; intro η. (* optional *)
-    unfold splay_spec. intros ??.
-    intros.
-    (* TODO: Add the following pattern into pure_rec_call *)
-    (* remember (l, x, r, ctx) as t. *)
-    (* replace ctx with t.2 by (rewrite Heqt; reflexivity). *)
-    (* replace l with (t.1.1.1) by (rewrite Heqt; reflexivity). *)
-    (* replace x with (t.1.1.2) by (rewrite Heqt; reflexivity). *)
-    (* replace r with (t.1.2) by (rewrite Heqt; reflexivity). *)
-    (* pure_rec t (fun _ : (tree A * A * tree A * zipper A) => True) (@splay_wf A). *)
-    (* do 3 destruct t as [t ?]. *)
-    eapply pure_rec_call with
-      (v:=(l, x, r, ctx))
-      (P:=fun _ => True)
-      (φ:= fun tuple =>
-             match tuple with
-             | (l, x, r, ctx) =>
-                 (fun t' => fringe t' = fringe (fill ctx (Node l x r))) end).
-    { apply splay_wf. }
-    { done. }
-    clear l x r ctx.
-    intros splay [[[l x] r] ctx] _ IH.
-    unfold zlt in IH.
-    (* Perform case analysis over the zipper [ctx]. *)
-    destruct ctx as [| ctx y ry | ly y ctx ]; pure1.
-    (* Case: [Root]. *)
-    {
-      (* Establish the postcondition. *)
-      prove_same_fringe. }
-    (* Case: [NodeL]. *)
-    { (* Perform case analysis on the second level of the zipper. *)
-      destruct ctx as [| up z rz | lz z up ];
-      pure1.
-      (* Subcase: [Root]. *)
-      { (* Establish the postcondition. *)
-        prove_same_fringe. }
-      (* Subcase: [NodeL]. *)
-      { (* Apply the induction hypothesis. *)
-        pure1. intros t' Ht'.
-        (* Establish the postcondition. *)
-        rewrite Ht'. prove_same_fringe. }
-      (* Subcase: [NodeR]. *)
-      { (* Apply the induction hypothesis. *)
-        pure1. intros t' Ht'.
-        (* Establish the postcondition. *)
-        rewrite Ht'.
-        prove_same_fringe. }
-    }
-    (* Case: [NodeR]. *)
-    { (* Perform case analysis on the second level of the zipper. *)
-      destruct ctx as [| up z rz | lz z up ]; pure1.
-      (* Subcase: [Root]. *)
-      {
-        (* Establish the postcondition. *)
-        prove_same_fringe. }
-      (* Subcase: [NodeL]. *)
-      {
-        (* Apply the induction hypothesis. *)
-        pure1. intros t' Ht'.
-        (* Establish the postcondition. *)
-        rewrite Ht'.
-        prove_same_fringe. }
-      (* Subcase: [NodeR]. *)
-      {
-        (* Apply the induction hypothesis. *)
-        pure1. intros t' Ht'.
-        (* Establish the postcondition. *)
-        rewrite Ht'.
-        prove_same_fringe. }
-    }
-  }
-  intros splay Hsplay. pure_continue.
+  trivial.
+Qed.
+(*   pure_specify "splay" splay_spec. *)
+(*   (* Subgoal: prove that [splay] satisfies its specification. *) *)
+(*   { generalize η; clear η; intro η. (* optional *) *)
+(*     unfold splay_spec. intros ??. *)
+(*     intros. *)
+(*     (* TODO: Add the following pattern into pure_rec_call *) *)
+(*     (* remember (l, x, r, ctx) as t. *) *)
+(*     (* replace ctx with t.2 by (rewrite Heqt; reflexivity). *) *)
+(*     (* replace l with (t.1.1.1) by (rewrite Heqt; reflexivity). *) *)
+(*     (* replace x with (t.1.1.2) by (rewrite Heqt; reflexivity). *) *)
+(*     (* replace r with (t.1.2) by (rewrite Heqt; reflexivity). *) *)
+(*     (* pure_rec t (fun _ : (tree A * A * tree A * zipper A) => True) (@splay_wf A). *) *)
+(*     (* do 3 destruct t as [t ?]. *) *)
+(*     eapply pure_rec_call with *)
+(*       (v:=(l, x, r, ctx)) *)
+(*       (P:=fun _ => True) *)
+(*       (φ:= fun tuple => *)
+(*              match tuple with *)
+(*              | (l, x, r, ctx) => *)
+(*                  (fun t' => fringe t' = fringe (fill ctx (Node l x r))) end). *)
+(*     { apply splay_wf. } *)
+(*     { done. } *)
+(*     clear l x r ctx. *)
+(*     intros splay [[[l x] r] ctx] _ IH. *)
+(*     unfold zlt in IH. *)
+(*     (* Perform case analysis over the zipper [ctx]. *) *)
+(*     destruct ctx as [| ctx y ry | ly y ctx ]; pure1. *)
+(*     (* Case: [Root]. *) *)
+(*     { *)
+(*       (* Establish the postcondition. *) *)
+(*       prove_same_fringe. } *)
+(*     (* Case: [NodeL]. *) *)
+(*     { (* Perform case analysis on the second level of the zipper. *) *)
+(*       destruct ctx as [| up z rz | lz z up ]; *)
+(*       pure1. *)
+(*       (* Subcase: [Root]. *) *)
+(*       { (* Establish the postcondition. *) *)
+(*         prove_same_fringe. } *)
+(*       (* Subcase: [NodeL]. *) *)
+(*       { (* Apply the induction hypothesis. *) *)
+(*         pure1. intros t' Ht'. *)
+(*         (* Establish the postcondition. *) *)
+(*         rewrite Ht'. prove_same_fringe. } *)
+(*       (* Subcase: [NodeR]. *) *)
+(*       { (* Apply the induction hypothesis. *) *)
+(*         pure1. intros t' Ht'. *)
+(*         (* Establish the postcondition. *) *)
+(*         rewrite Ht'. *)
+(*         prove_same_fringe. } *)
+(*     } *)
+(*     (* Case: [NodeR]. *) *)
+(*     { (* Perform case analysis on the second level of the zipper. *) *)
+(*       destruct ctx as [| up z rz | lz z up ]; pure1. *)
+(*       (* Subcase: [Root]. *) *)
+(*       { *)
+(*         (* Establish the postcondition. *) *)
+(*         prove_same_fringe. } *)
+(*       (* Subcase: [NodeL]. *) *)
+(*       { *)
+(*         (* Apply the induction hypothesis. *) *)
+(*         pure1. intros t' Ht'. *)
+(*         (* Establish the postcondition. *) *)
+(*         rewrite Ht'. *)
+(*         prove_same_fringe. } *)
+(*       (* Subcase: [NodeR]. *) *)
+(*       { *)
+(*         (* Apply the induction hypothesis. *) *)
+(*         pure1. intros t' Ht'. *)
+(*         (* Establish the postcondition. *) *)
+(*         rewrite Ht'. *)
+(*         prove_same_fringe. } *)
+(*     } *)
+(*   } *)
+(*   intros splay Hsplay. pure_continue. *)
 
-  pure_specify "splay_leaf" splay_leaf_spec.
-  (* Subgoal: prove that [splay_leaf] satisfies its specification. *)
-  { unfold splay_leaf_spec. intros.
-    (* This helps Coq recognize the encoding of [Leaf] at type [A]. *)
-    (* Without this, the tactic [encode] fails to solve [Leaf = #?t]. TODO *)
-    pose proof (@solve_encode_Leaf A _).
-    (* Step into the function. *)
-    pure_enter. fixme.
-    (* Perform case analysis over the zipper [ctx]. *)
-    destruct ctx as [| up x r | r x up ]; pure1.
-    (* Case: [Root]. *)
-    { prove_same_fringe. }
-    (* Case: [NodeL]. *)
-    { pure0. }
-    (* Case: [NodeR]. *)
-    { pure0. }
-  }
-  intros splay_leaf Hsplay_leaf. pure_continue.
+(*   pure_specify "splay_leaf" splay_leaf_spec. *)
+(*   (* Subgoal: prove that [splay_leaf] satisfies its specification. *) *)
+(*   { unfold splay_leaf_spec. intros. *)
+(*     (* This helps Coq recognize the encoding of [Leaf] at type [A]. *) *)
+(*     (* Without this, the tactic [encode] fails to solve [Leaf = #?t]. TODO *) *)
+(*     pose proof (@solve_encode_Leaf A _). *)
+(*     (* Step into the function. *) *)
+(*     pure_enter. fixme. *)
+(*     (* Perform case analysis over the zipper [ctx]. *) *)
+(*     destruct ctx as [| up x r | r x up ]; pure1. *)
+(*     (* Case: [Root]. *) *)
+(*     { prove_same_fringe. } *)
+(*     (* Case: [NodeL]. *) *)
+(*     { pure0. } *)
+(*     (* Case: [NodeR]. *) *)
+(*     { pure0. } *)
+(*   } *)
+(*   intros splay_leaf Hsplay_leaf. pure_continue. *)
 
-  pure_specify "zlookup" zlookup_spec.
-  (* Subgoal: prove that [zlookup] satisfies its specification. *)
-  { unfold zlookup_spec. do 4 intro.
-    intros Hcompare ??? Hbst.
-    eapply pure_rec_call_unary with
-      (v:=(t,x,ctx))
-      (P:=fun '(t, _, _) => bst (strict le) t)
-      (φ:=fun tuple =>
-            match tuple with
-            | (t, x, ctx) =>
-                λ '(oy, t'),
-                member le x (fringe t) oy ∧ fringe t' = fringe (fill ctx t)
-            end).
-    { apply zlookup_wf. }
-    { apply Hbst. }
-    clear dependent t x ctx.
-    intros vf [[t x] ctx] Hbst IH.
-    (* Reason by induction on the tree [t]. *)
-    destruct t as [|l y r]; pure1.
-    (* Case: [Leaf]. *)
-    { intros t' Ht'. pure1.
-      (* Establish the postcondition: *)
-      split.
-      - simpl member. intros. rewrite elem_of_nil. tauto. (* TODO use [set_solver]? *)
-      - assumption. }
-    (* Case: [Node]. *)
-    { (* The call [compare x y] is curried. *)
-      intros v Hv.
-      eapply pure_bind. (* TODO try to automate this *)
-      { eapply Hv. }
-      clear v Hv.
-      intros c Hc. cbn in Hc.
-      (* The call [compare x y] is now complete. *)
-      destruct_bst_Node.
-      pure_continue.
-      rewrite lt_repr_repr; [ | representable | representable].
-      assert (c < 0 ∨ 0 < c ∨ c = 0) as [|[|]] by lia.
-      (* Case: [c < 0], that is, [x < y]. *)
-      { rewrite ltb_true; [ | lia ].
-        pure1. eapply pure_consequence.
-        { eapply IH; eauto.
-          { unfold tlt. simpl; lia. }}
-        intros [ox t'] (? & ?); simpl.
-        (* Establish the postcondition: *)
-        split.
-        - rewrite bst_member_left; representable.
-        - assumption. }
-      (* Case: [c > 0], that is, [x > y]. *)
-      { rewrite ltb_false; try lia.
-        pure1.
-        rewrite lt_repr_repr; representable.
-        rewrite ltb_true; try lia.
-        pure1. eapply pure_consequence.
-        { eapply IH; first assumption.
-          { unfold tlt. simpl; lia. }}
-        intros [b t'] (? & ?); simpl.
-        (* Establish the postcondition: *)
-        split.
-        - rewrite bst_member_right; representable.
-        - assumption. }
-      (* Subcase: [c = 0], so [x] and [y] are equivalent with respect to
-         the preorder [le]. *)
-      { rewrite ltb_false; try lia.
-        pure1.
-        rewrite lt_repr_repr; representable.
-        rewrite ltb_false; try lia.
-        pure1.
-        intros t' Ht'. pure1.
-        (* Establish the postcondition: *)
-        assert (equivalent le x y) by tauto.
-        split; [ split |]; simpl.
-        - assumption.
-        - rewrite !elem_of_app elem_of_list_singleton. tauto.
-        - assumption. }
-    }
-  }
-  intros zlookup zlookup_spec. pure_continue. pure_continue.
+(*   pure_specify "zlookup" zlookup_spec. *)
+(*   (* Subgoal: prove that [zlookup] satisfies its specification. *) *)
+(*   { unfold zlookup_spec. do 4 intro. *)
+(*     intros Hcompare ??? Hbst. *)
+(*     eapply pure_rec_call_unary with *)
+(*       (v:=(t,x,ctx)) *)
+(*       (P:=fun '(t, _, _) => bst (strict le) t) *)
+(*       (φ:=fun tuple => *)
+(*             match tuple with *)
+(*             | (t, x, ctx) => *)
+(*                 λ '(oy, t'), *)
+(*                 member le x (fringe t) oy ∧ fringe t' = fringe (fill ctx t) *)
+(*             end). *)
+(*     { apply zlookup_wf. } *)
+(*     { apply Hbst. } *)
+(*     clear dependent t x ctx. *)
+(*     intros vf [[t x] ctx] Hbst IH. *)
+(*     (* Reason by induction on the tree [t]. *) *)
+(*     destruct t as [|l y r]; pure1. *)
+(*     (* Case: [Leaf]. *) *)
+(*     { intros t' Ht'. pure1. *)
+(*       (* Establish the postcondition: *) *)
+(*       split. *)
+(*       - simpl member. intros. rewrite elem_of_nil. tauto. (* TODO use [set_solver]? *) *)
+(*       - assumption. } *)
+(*     (* Case: [Node]. *) *)
+(*     { (* The call [compare x y] is curried. *) *)
+(*       intros v Hv. *)
+(*       eapply pure_bind. (* TODO try to automate this *) *)
+(*       { eapply Hv. } *)
+(*       clear v Hv. *)
+(*       intros c Hc. cbn in Hc. *)
+(*       (* The call [compare x y] is now complete. *) *)
+(*       destruct_bst_Node. *)
+(*       pure_continue. *)
+(*       rewrite lt_repr_repr; [ | representable | representable]. *)
+(*       assert (c < 0 ∨ 0 < c ∨ c = 0) as [|[|]] by lia. *)
+(*       (* Case: [c < 0], that is, [x < y]. *) *)
+(*       { rewrite ltb_true; [ | lia ]. *)
+(*         pure1. eapply pure_consequence. *)
+(*         { eapply IH; eauto. *)
+(*           { unfold tlt. simpl; lia. }} *)
+(*         intros [ox t'] (? & ?); simpl. *)
+(*         (* Establish the postcondition: *) *)
+(*         split. *)
+(*         - rewrite bst_member_left; representable. *)
+(*         - assumption. } *)
+(*       (* Case: [c > 0], that is, [x > y]. *) *)
+(*       { rewrite ltb_false; try lia. *)
+(*         pure1. *)
+(*         rewrite lt_repr_repr; representable. *)
+(*         rewrite ltb_true; try lia. *)
+(*         pure1. eapply pure_consequence. *)
+(*         { eapply IH; first assumption. *)
+(*           { unfold tlt. simpl; lia. }} *)
+(*         intros [b t'] (? & ?); simpl. *)
+(*         (* Establish the postcondition: *) *)
+(*         split. *)
+(*         - rewrite bst_member_right; representable. *)
+(*         - assumption. } *)
+(*       (* Subcase: [c = 0], so [x] and [y] are equivalent with respect to *)
+(*          the preorder [le]. *) *)
+(*       { rewrite ltb_false; try lia. *)
+(*         pure1. *)
+(*         rewrite lt_repr_repr; representable. *)
+(*         rewrite ltb_false; try lia. *)
+(*         pure1. *)
+(*         intros t' Ht'. pure1. *)
+(*         (* Establish the postcondition: *) *)
+(*         assert (equivalent le x y) by tauto. *)
+(*         split; [ split |]; simpl. *)
+(*         - assumption. *)
+(*         - rewrite !elem_of_app elem_of_list_singleton. tauto. *)
+(*         - assumption. } *)
+(*     } *)
+(*   } *)
+(*   intros zlookup zlookup_spec. pure_continue. pure_continue. *)
 
-  (* Conclude. *)
-  tauto.
+(*   (* Conclude. *) *)
+(*   tauto. *)
 
-Time Qed.
+(* Time Qed. *)
