coq-osiris/theories/proofmode/examples_wp.v
@@ -5,7 +5,6 @@ From iris.prelude Require Import options.
 Import uPred.
 
 From osiris Require Import osiris.
-Local Transparent eval.
 
 Context `{!osirisGS Σ}.
 
@@ -21,7 +20,6 @@ Proof.
   (* This goal is false: the variable [y] is unbound. *)
   iIntros.
   wp.
-  wp_continue.
 Abort. (* expected *)
 
 (* let x = (A (), B ()) in let (x1, x2) = x in x1 *)
@@ -35,7 +33,7 @@ Definition example :=
 
 Goal ⊢ WP (eval [] example) {{ RET v, ⌜v = VConstant "A"⌝ }}.
 Proof.
-  wp. do 2 wp_continue.
+  wp. wp. wp.
   iPureIntro. reflexivity.
 Qed.
 
@@ -51,8 +49,7 @@ Goal
   let env := [("z1", v1); ("z2", v2)] in
   ⊢ WP (eval env example2) {{ RET v, ⌜v = v1⌝ }}.
 Proof.
-  iIntros. wp.
-  do 2 wp_continue.
+  iIntros. wp. wp. wp.
   iPureIntro. reflexivity.
 Qed.
 
@@ -118,25 +115,17 @@ Lemma spec_example4:
     {{ RET v, ⌜v = VPair (VConstant "A") (VConstant "A")⌝ }}.
 Proof.
   unfold example4.
-  wp. wp_bind.
+  wp.
   (* The environment is about to be extended with a binding of the variable
      "id" to a certain closure. Now is the time to prove a specification
      for this closure; then, we can make this closure opaque. *)
-  oSpecify "id" spec_id vid "#Hid".
+  oSpecify "id" spec_id id "#Hid".
   (* Subgoal: prove that [fun x -> x] satisfies [spec_id]. *)
   { unfold spec_id. iModIntro. iIntros (v). wp. equality. }
   (* The variable "id" is now bound to an abstract closure [id]. *)
-
-  (* Abstract away [example3]; its spec suffices. *)
-  (* TODO this is broken; [example3] has been unfolded/simplified already
-  generalize example3 spec_example3.
-  intros example3 Hexample3.
-  (* Attack the goal. *)
-  wp_continue.
-  iApply wp_simp; [ simp_really |]. (* TODO [wp] should do this *)
-  wp_use Hexample3.
-  wp_use "Hid". *)
-Abort.
+  iApply spec_example3.
+  wp_use "Hid".
+Qed.
 
 (* An example that involves an assertion. *)
 
@@ -149,20 +138,7 @@ Proof.
   (* TODO make [choose] opaque somewhere else *)
   (* TODO and prove a [wp] rule for [eval (EAssert _)]
           so we do not need to descend to the level of [choose] *)
-  Opaque choose.
-  wp.
-  (* Applying [wp_bind] (unary) followed with [wp_choose_ok]
-     duplicates the proof of the continuation. We must use
-     [wp_bind_binary] to introduce a cut and avoid duplication. *)
-  iApply wp_bind_binary.
-  + iApply (wp_choose_ok _ (True)%I).
-    - auto.
-    - iModIntro. iIntros "_". wp. auto.
-  + iSimpl. iIntros (??).
-    (* TODO not clean! *)
-    unfold lift_ipure. destruct v.
-    - wp. equality.
-    - elim_void e.
+  by wp.
 Qed.
 
 (* let id = identity in
@@ -176,13 +152,14 @@ Definition example4b :=
 Lemma spec_example4b:
   ⊢ WP eval [] example4b {{ RET v, ⌜v = VUnit⌝ }}.
 Proof.
-  unfold example4b. wp. wp_bind.
+  unfold example4b.
+  wp.
   (* Deal with the local binding of [id]. *)
   oSpecify "id" spec_id vid "#Hid".
   { unfold spec_id. iIntros (v).
     iModIntro. wp. equality. }
   (* We are looking at [id id]. *)
-  wp_bind. wp_use "Hid".
+  wp. wp_bind. wp_use "Hid".
   wp_pure_postcondition; subst.
   wp_use "Hid".
 Qed.
@@ -198,13 +175,13 @@ Definition example4c :=
 Lemma spec_example4c:
   ⊢ WP eval [] example4c {{ RET v, ⌜v = VUnit⌝}}.
 Proof.
-  unfold example4c. wp. wp_bind.
+  unfold example4c. wp.
   (* Deal with the local binding of [id]. *)
   oSpecify "id" spec_id vid "#Hid".
   { unfold spec_id. iIntros (v).
     iModIntro. wp. equality. }
   (* We are looking at [id()]. *)
-  wp_bind. wp_use "Hid".
+  wp. wp_bind. wp_use "Hid".
   wp_pure_postcondition.
   (* We are again looking at [id()]. *)
   wp_use "Hid".
@@ -221,13 +198,15 @@ Definition example4d :=
 Lemma spec_example4d:
   ⊢ WP eval [] example4d {{ RET v, ⌜v = VUnit⌝}}.
 Proof.
-  unfold example4d. wp. wp_bind.
+  unfold example4d. wp.
   (* Deal with the local binding of [id]. *)
   oSpecify "id" spec_id vid "#Hid".
   { unfold spec_id. iIntros (v).
     iModIntro. wp. equality. }
-  (* Here, [wp] is unable to make progress because we are looking at two
+  wp.
+  (* Here, [wp] is no longer able to make progress because we are looking at two
      function calls in parallel. *)
+
   wp_par; try wp_absurd.
 
   (* id id *)
@@ -298,39 +277,7 @@ Lemma spec_walk_example_concrete :
   ⊢ WP eval [] (walk_example e) {{ RET v, ⌜v = encode tt⌝ }}.
 Proof.
   (* The code is pure and terminating and can be fully evaluated. *)
-  iIntros. wp. wp_continue. equality.
-Qed.
-
-(* The following example illustrates how to reason about a local function.
-   When the environment is about to be extended with a binding of the
-   variable "walk" to a closure, we prove a specification for this closure,
-   then we make this closure opaque. *)
-Lemma spec_walk_example_abstract :
-  forall (bs : list bool),
-  let η := [("xs", (encode bs))] in
-  ⊢ WP (eval η (walk_example (EVar "xs"))) {{ RET v, ⌜v = encode tt⌝ }}.
-Proof.
-  intros. wp. wp_bind.
-  (* The environment is about to be extended with a binding of the variable
-     "walk" to a certain closure. Now is the time to prove a specification
-     for this closure; then, we can make this closure opaque. *)
-  oSpecify "walk" spec_walk vid "#Hwalk".
-  (* Subgoal: prove that the closure satisfies [spec_walk]. *)
-  { (* The environment [η] is irrelevant, since the code is in fact closed.
-       Abstract it away. *)
-    generalize η. clear bs η. intros η.
-    unfold spec_walk.
-    (* Prove the spec by induction on the list [bs]. *)
-    iIntros "!>"(bs).
-    iInduction bs as [| b bs ] "IHbs";
-    wp_enter_and_abstract; iIntros (walk); wp.
-    { cbn. wp. equality. }
-    { wp_use "IHbs". wp_pure_postcondition. wp.
-      equality. }
-  }
-  (* The variable "walk" is now bound to an abstract closure [walk]. *)
-  (* The remains to exploit the hypothesis [Hwalk]. *)
-  wp_use "Hwalk".
+  iIntros. wp. wp. equality.
 Qed.
 
 (* ------------------------------------------------------------------------- *)
@@ -377,6 +324,20 @@ Qed.
    !l
  *)
 
+
+
+Local Ltac wp_progress :=
+  first [
+      lazymatch goal with
+      | |- environments.envs_entails _ $ wp _ _ (eval _ ?e) _ =>
+          rewrite eval_eval'; try progress wp_cbn
+      end
+    | wp_cbn (* TODO: better control the reduction strategy. *)
+    | progress wp_simp
+    | cbn beta delta -[app]
+    ].
+
+
 Definition ref_store_load: expr :=
   ELet1Var "l" (ERef (EConstant "A")) $
   ELet1Var "_" (EStore (EVar "l") (EConstant "B")) $
@@ -384,10 +345,9 @@ Definition ref_store_load: expr :=
 
 Goal ⊢ WP (eval [] ref_store_load) {{ RET v, ⌜ v = VConstant "B" ⌝ }}.
 Proof.
-  unfold ref_store_load.
   wp.
-  wp_alloc l "[Hl _]". wp_continue.
-  wp_store "Hl". wp_continue.
+  wp_alloc l "[Hl _]".
+  wp_store "Hl".
   wp_load "Hl".
   iPureIntro. reflexivity.
 Qed.
@@ -418,41 +378,66 @@ Definition simple_module_spec: val → iProp Σ :=
 .
 
 
-Goal
-  ⊢ WP eval_mexpr [] simple_module {{ RET v, simple_module_spec v }}.
-Proof.
-  wp. wp_bind.
+Local Ltac wp_setup :=
+  iStartProof;
+  lazymatch goal with
+  | |- environments.envs_entails ?Δ $ wp _ _ _ _ =>
+      let Δ :=
+        eval cbn in (environments.env_to_list
+                       (environments.env_intuitionistic Δ)) in
+      let rec lookforme l :=
+        lazymatch constr:(l) with
+        | [] => idtac
+        | (satisfies_spec ?Λ0 ?v) :: ?t =>
+            let Λ := eval hnf in Λ0 in
+            lazymatch constr:(Λ) with
+            | SpecModule Auto ?l ?P =>
+                lazymatch goal with
+                | _ : pure_spec Λ0 v |- _ => idtac
+                | _ =>
+                    iPoseProof ((satisfies_pure_spec Λ v) with "[$]")
+                    as "%";
+                    change Λ with Λ0 in *
+                end
+            | _ => idtac
+            end ; lookforme t
+        | _ :: ?t => lookforme t
+        end in
+      lookforme Δ
+  end
+.
 
-  (* [f] is about to be added to the environment *)
-  oSpecify "f" spec_id vf "#Hid".
-  { iIntros(v). iModIntro. wp. equality. }
 
-  wp_bind.
+(* Goal *)
+(*   ⊢ WP eval_mexpr [] simple_module {{ RET v, simple_module_spec v }}. *)
+(* Proof. *)
+(*   wp. *)
+(*   (* [f] is about to be added to the environment *) *)
+(*   oSpecify "f" spec_id vf "#Hid". *)
+(*   { iIntros(v). iModIntro. wp. equality. } *)
 
-  (* [g] is about to be added to the environment *)
-  oSpecify "g" spec_id vg "#Hid'".
-  { iIntros(v). iModIntro.
-    wp_use "Hid". }
+(*   wp_bind. *)
 
-  (* We can use the spec of [f] at the function call (of the body of [h]). *)
-  wp_bind. wp_use "Hid". wp_pure_postcondition; subst; cbn.
-  wp_bind. wp_concat. wp.
+(*   (* [g] is about to be added to the environment *) *)
+(*   oSpecify "g" spec_id vg "#Hid'". *)
+(*   { iIntros(v). iModIntro. *)
+(*     wp_use "Hid". } *)
 
-  (* Proving the trivial post condition using the aforementioned specs. *)
-  wp_module_spec.
-Qed.
+(*   (* We can use the spec of [f] at the function call (of the body of [h]). *) *)
+(*   wp_bind. wp_use "Hid". wp_pure_postcondition; subst; cbn. *)
+(*   wp_bind. wp_concat. wp. *)
+
+(*   (* Proving the trivial post condition using the aforementioned specs. *) *)
+(*   wp_module_spec. *)
+(* Qed. *)
 
 (* -------------------------------------------------------------------------- *)
 
 (* Test : specify the body of a function instead of the function itself. *)
 
-From osiris.proofmode Require Import proofmode.
-
 (* ( (x * z) + (y * t) ) + v*)
 Definition test_innerbody x y z t v  : expr :=
-  EIntAdd
-    (EIntAdd (EIntMul (EVar x) (EVar z)) (EIntMul (EVar y) (EVar t)))
-    (EVar v).
+  ((EVar x) * (EVar z) + (EVar y) * (EVar t) + (EVar v))%expr.
 Opaque test_innerbody.
 
 Definition test_body : expr :=
@@ -496,5 +481,5 @@ Definition add_uc : expr :=
 Lemma add_test (i j: Z) :
   ⊢ WP eval [("bloup", #0%Z)] add_uc {{ RET v, ⌜ v = #16 ⌝ }}.
 Proof.
-  wp. wp_continue. equality.
+  wp. wp. equality.
 Qed.
